src/test/dafny/proofs/Transient.dfy
@@ -32,10 +32,10 @@ module Transient {
     // makes an arbitrary call.  Once this is complete, the lock is released.
     // The key property is that a successful call to this contract increments
     // storage[0] at most once.
-    const LOCK_CONTRACT := Code.Create(
+    const LOCK_CONTRACT : seq<u8> :=
     [
         // If TSTORAGE[0] != 0 then REVERT  
-        PUSH0, TLOAD, PUSH1, 0x1d, JUMPI,
+        PUSH0, TLOAD, PUSH2, 0x00, 0x1e , JUMPI,
         // Set TSTORAGE[0]=1
         PUSH1, 0x01, PUSH0, TSTORE,
         // Increment STORAGE[0]
@@ -48,94 +48,187 @@ module Transient {
         STOP,
         // Revert
         JUMPDEST, PUSH0, PUSH0, REVERT
-        ]
-    )
+    ]    
 
-     /**
-     *  Simple proof about the lock contract
-     */
-    method {:only} lock_proof(st: ExecutingState) returns (st': State)
-        /** Initial state with PC = 0 and empty stack. */
-        requires st.PC() == 0 && st.Operands() == 0 && st.Fork() == EvmFork.BERLIN
-        /** Enough gas. */
-        requires st.Gas() >= 40000
-        /** Permission to write to storage. */
-        requires st.WritesPermitted()
-        /** Code is LOCK_CONTRACT. */
-        requires st.evm.code == LOCK_CONTRACT
-        /** This evm context cannot change */
-        ensures st'.EXECUTING? ==> st'.evm.context == st.evm.context
-        /** This account must still exist */
-        ensures st'.RETURNS? ==> st.evm.context.address in st'.world.accounts.Keys
-        /** If it terminates normally, then storage[0] incremented by 1*/
-        // ensures st'.RETURNS? && (st.Load(0) as nat) < MAX_U256 ==> st'.world.Read(st.evm.context.address,0) == st.Load(0) + 1
-        // ensures st'.RETURNS? && (st.Load(0) as nat) == MAX_U256 ==> st'.world.Read(st.evm.context.address,0) == 0
-        /** If it terminates normally, then lock was acquired */
-        // ensures st'.RETURNS? ==> st.TransientLoad(0) == 0
-        /** If it terminates normally, then lock is released */
-        // ensures st'.RETURNS? ==> st'.transient.Read(st.evm.context.address,0) == 0
+    method block_0_0x0000(st': EvmState.ExecutingState) returns (st'': EvmState.State)
+    requires st'.evm.code == Code.Create(LOCK_CONTRACT)
+    requires st'.WritesPermitted() && st'.PC() == 0x0000 && st'.Gas() <= (MAX_U256 as nat)
+    // Stack height(s)
+    requires st'.Operands() == 0
+    // This evm context cannot change
+    ensures st''.EXECUTING? ==> st''.evm.context == st'.evm.context
+    // This account must still exist
+    ensures st''.RETURNS? ==> st'.evm.context.address in st''.world.accounts.Keys
+    // If it terminates normally, then storage[0] incremented by 1
+    ensures st''.RETURNS? && (st'.Load(0) as nat) < MAX_U256 ==> st''.world.Read(st'.evm.context.address,0) == st'.Load(0) + 1
+    ensures st''.RETURNS? && (st'.Load(0) as nat) == MAX_U256 ==> st''.world.Read(st'.evm.context.address,0) == 0
+    // If it terminates normally, then lock was available (i.e. not acquired)
+    ensures st''.RETURNS? ==> !LockAcquired(st', st'.evm.context.address)
+    // If it terminates normally, then lock is released
+    ensures st''.RETURNS? ==> st''.transient.Read(st'.evm.context.address,0) == 0
     {
-        st' := st;
-        // If TSTORAGE[0] != 0 then REVERT  
-        st' := Push0(st');
-        st' := TLoad(st');
-        var lock := st'.Peek(0);
-        st' := Push1(st',0x1d);
-        assume {:axiom} st.IsJumpDest(0x1d);
-        st' := JumpI(st');        
-        if st'.PC() == 0x1d {
-            assert lock != 0;
-            st' := Push0(st');
-            st' := Push0(st');
-            st' := Revert(st');
-        } else {
-            assert lock == 0;
-            st' := JumpDest(st');
-            // Set TSTORAGE[0]=1
-            st' := Push1(st',1);
-            st' := Push0(st');
-            st' := TStore(st');
-            // Increment STORAGE[0]
-            st' := Push0(st');
-            st' := SLoad(st');
-            st' := Push1(st',0x1);
-            st' := Add(st');
-            st' := Push0(st');
-            st' := SStore(st');            
-            // Prepare arguments
-            st' := Push0(st');
-            st' := Push0(st');
-            st' := Push0(st');
-            st' := Push0(st');
-            st' := Push0(st');
-            st' := Push0(st');
-            st' := CallDataLoad(st');
-            st' := Bytecode.Gas(st');
-            assert st'.EXECUTING?;
-            // >>> Contract call starts here
-            var CONTINUING(cc) := Bytecode.Call(st');
-            {
-                var inner := cc.CallEnter(1);
-                inner := randomContract(inner, st'.evm.context.address);
-                st' := cc.CallReturn(inner);
-            } // <<< Contract call ends here
-            // Handle call failure
-            if st'.EXECUTING? {
-                // Set TSTORAGE[0]=0
-                st' := Push0(st');
-                st' := Push0(st');
-                st' := TStore(st');
-                // Success!
-                st' := Stop(st');
-            }
-        } 
+        var st := st';
+        //|fp=0x0000||
+        st := Push0(st);
+        //|fp=0x0000|0x00|
+        st := TLoad(st);
+        //|fp=0x0000|_|
+        st := Push2(st,0x001e);
+        //|fp=0x0000|0x1e,_|
+        assume {:axiom} st.IsJumpDest(0x1e);
+        st := JumpI(st);
+        if st.PC() == 0x1e { st := block_0_0x001e(st); return st;}
+        //|fp=0x0000||
+        st := Push1(st,0x01);
+        //|fp=0x0000|0x01|
+        st := Push0(st);
+        //|fp=0x0000|0x00,0x01|
+        st := TStore(st);
+        //|fp=0x0000||
+        st := Push0(st);
+        st := block_0_0x000b(st);
+        return st;
     }
 
-    method randomContract(vm:EvmState.ExecutingState, lockAccount: u160) returns (vm':EvmState.State) 
-    requires vm.world.Exists(lockAccount)
-    ensures vm.world.GetAccount(lockAccount) == vm'.world.GetAccount(lockAccount)
+    method block_0_0x000b(st': EvmState.ExecutingState) returns (st'': EvmState.State)
+    requires st'.evm.code == Code.Create(LOCK_CONTRACT)
+    requires st'.WritesPermitted() && st'.PC() == 0x000b && st'.Gas() <= (MAX_U256 as nat)
+    // Stack height(s)
+    requires st'.Operands() == 1
+    // Static stack items
+    requires (st'.Peek(0) == 0x0)
+    // Lock must be acquired
+    requires LockAcquired(st', st'.evm.context.address)
+    // This evm context cannot change
+    ensures st''.EXECUTING? ==> st''.evm.context == st'.evm.context
+    // This account must still exist
+    ensures st''.RETURNS? ==> st'.evm.context.address in st''.world.accounts.Keys
+    // If it terminates normally, then storage[0] incremented by 1
+    ensures st''.RETURNS? && (st'.Load(0) as nat) < MAX_U256 ==> st''.world.Read(st'.evm.context.address,0) == st'.Load(0) + 1
+    ensures st''.RETURNS? && (st'.Load(0) as nat) == MAX_U256 ==> st''.world.Read(st'.evm.context.address,0) == 0
+    // If it terminates normally, then lock is released
+    ensures st''.RETURNS? ==> st''.transient.Read(st'.evm.context.address,0) == 0
     {
-        // This implementation is arbitrary.
-        return vm;
+        var st := st';
+        //|fp=0x0000|0x00|
+        st := SLoad(st);
+        //|fp=0x0000|_|
+        st := Push1(st,0x01);
+        //|fp=0x0000|0x01,_|
+        st := Add(st);
+        //|fp=0x0000|_|
+        st := Push0(st);
+        //|fp=0x0000|0x00,_|
+        st := SStore(st);
+        //|fp=0x0000||
+        st := Push0(st);
+        //|fp=0x0000|0x00|
+        st := Push0(st);
+        //|fp=0x0000|0x00,0x00|
+        st := Push0(st);
+        st := block_0_0x0014(st);
+        return st;
+    }
+
+    method block_0_0x0014(st': EvmState.ExecutingState) returns (st'': EvmState.State)
+    requires st'.evm.code == Code.Create(LOCK_CONTRACT)
+    requires st'.WritesPermitted() && st'.PC() == 0x0014 && st'.Gas() <= (MAX_U256 as nat)
+    // Stack height(s)
+    requires st'.Operands() == 3
+    // Static stack items
+    requires (st'.Peek(0) == 0x0 && st'.Peek(1) == 0x0 && st'.Peek(2) == 0x0)
+    // Lock must be acquired
+    requires LockAcquired(st', st'.evm.context.address)
+    // This evm context cannot change
+    ensures st''.EXECUTING? ==> st''.evm.context == st'.evm.context
+    // This account must still exist
+    ensures st''.RETURNS? ==> st'.evm.context.address in st''.world.accounts.Keys
+    // No change to storage[0]
+    ensures st''.RETURNS? ==> st''.world.Read(st'.evm.context.address,0) == st'.Load(0)
+    // If it terminates normally, then lock is released
+    ensures st''.RETURNS? ==> st''.transient.Read(st'.evm.context.address,0) == 0
+    {
+        var st := st';
+        //|fp=0x0000|0x00,0x00,0x00|
+        st := Push0(st);
+        //|fp=0x0000|0x00,0x00,0x00,0x00|
+        st := Push0(st);
+        //|fp=0x0000|0x00,0x00,0x00,0x00,0x00|
+        st := Push0(st);
+        //|fp=0x0000|0x00,0x00,0x00,0x00,0x00,0x00|
+        st := CallDataLoad(st);
+        //|fp=0x0000|_,0x00,0x00,0x00,0x00,0x00|
+        st := Bytecode.Gas(st);
+        //|fp=0x0000|_,_,0x00,0x00,0x00,0x00,0x00|
+        var CONTINUING(cc) := Bytecode.Call(st);
+        {
+            var inner := cc.CallEnter(1);
+            if inner.EXECUTING? { inner := external_call(cc.sender,inner); }
+            st := cc.CallReturn(inner);
+        }
+        //|fp=0x0000|_|
+        st := Push0(st);
+        //|fp=0x0000|0x00,_|
+        st := Push0(st);
+        st := block_0_0x001c(st);
+        return st;
+    }
+
+    method block_0_0x001c(st': EvmState.ExecutingState) returns (st'': EvmState.State)
+    requires st'.evm.code == Code.Create(LOCK_CONTRACT)
+    requires st'.WritesPermitted() && st'.PC() == 0x001c
+    // Stack height(s)
+    requires st'.Operands() == 3
+    // Static stack items
+    requires (st'.Peek(0) == 0x0 && st'.Peek(1) == 0x0)
+    // This evm context cannot change
+    ensures st''.RETURNS?
+    // This account must still exist
+    ensures st'.evm.context.address in st''.world.accounts.Keys
+    // No change to storage[0]
+    ensures st''.world.Read(st'.evm.context.address,0) == st'.Load(0)
+    // If it terminates normally, then lock is released
+    ensures st''.RETURNS? ==> st''.transient.Read(st'.evm.context.address,0) == 0
+    {
+        var st := st';
+        //|fp=0x0000|0x00,0x00,_|
+        st := TStore(st);
+        //|fp=0x0000|_|
+        st := Stop(st);
+        return st;
+    }
+
+    method block_0_0x001e(st': EvmState.ExecutingState) returns (st'': EvmState.State)
+    requires st'.evm.code == Code.Create(LOCK_CONTRACT)
+    requires st'.WritesPermitted() && st'.PC() == 0x001e
+    // Stack height(s)
+    requires st'.Operands() == 0
+    // Resulting state always an error
+    ensures st''.ERROR?
+    {
+        var st := st';
+        //|fp=0x0000||
+        st := JumpDest(st);
+        //|fp=0x0000||
+        st := Push0(st);
+        //|fp=0x0000|0x00|
+        st := Push0(st);
+        //|fp=0x0000|0x00,0x00|
+        st := Revert(st);
+        return st;
+    }
+
+    method external_call(sender: u160, st: EvmState.ExecutingState) returns (st':EvmState.TerminatedState)
+    requires st.Exists(sender)
+    // If successful return, account must still exist
+    ensures st'.RETURNS? ==> st'.world.Exists(sender) 
+    // If the sender's lock was acquired, then its account does not change.
+    ensures (st'.RETURNS? && LockAcquired(st,sender)) ==> st.GetAccount(sender) == st'.world.GetAccount(sender) {
+        return EvmState.ERROR(EvmState.INSUFFICIENT_GAS); // dummy
+    }
+
+    // Helper function to make reading the above easier.
+    function LockAcquired(st: EvmState.ExecutingState, account: u160) : bool {
+        st.evm.transient.Read(account,0) != 0
     }
 }
